lazy2
git-svn-id: svn://scm.gforge.inria.fr/svn/cfml@7 ba02c806-7d2b-4818-9a48-35b22e6bdc79

okasaki/LazyPairingHeap_proof.v
@@ -4,6 +4,24 @@ Require Import OrderedSig_ml HeapSig_ml OrderedSig_proof HeapSig_proof.
 Require Import LazyPairingHeap_ml.
 
 
+Instance union_inst : forall A, BagCard (multiset A).
+Admitted.
+
+Class Card_empty `{BagEmpty T, BagCard T} :=
+  { card_empty : card \{} = 0%nat }.
+Class Card_single `{BagSingle A T, BagCard T} :=
+  { card_single : forall X, card \{X} = 1%nat }.
+Class Card_union `{BagUnion T, BagCard T} :=
+  { card_union : forall E F, card (E \u F) = (card E + card F)%nat }.
+
+Instance card_empty_inst : forall A, Card_empty (T:=multiset A).
+Admitted.
+Instance card_single_inst : forall A, Card_single (T:=multiset A).
+Admitted.
+Instance card_union_inst : forall A, Card_union (T:=multiset A).
+Admitted.
+
+
 Module LazyPairingHeapSpec (O:MLOrdered) (OS:OrderedSigSpec with Module O:=O)
   <: HeapSigSpec with Definition H.MLElement.t := O.t.
 
@@ -76,6 +94,27 @@ Proof. apply empty_cf. xret~. Qed.
 
 Hint Extern 1 (RegisterSpec empty) => Provide empty_spec.
 
+Definition rep_spec_2 (a1 a2 A1 A2 B : Type)
+  (rep1:a1->A1->Prop) (rep2:a2->A2->Prop)
+  (RK:a1->a2->A1->A2->~~B->Prop) f :=
+  spec_2 (B:=B) (fun x1 x2 R => forall X1 X2, 
+    rep1 x1 X1 -> rep2 x2 X2 -> RK x1 x2 X1 X2 R) f.
+
+Definition rep_spec_2_hyp (a1 a2 A1 A2 B : Type)
+  (rep1:a1->A1->Prop) (rep2:a2->A2->Prop) (P:A1->A2->Prop)
+  (RK:a1->a2->A1->A2->~~B->Prop) f :=
+  spec_2 (B:=B) (fun x1 x2 R => forall X1 X2, 
+    rep1 x1 X1 -> rep2 x2 X2 -> P X1 X2 -> RK x1 x2 X1 X2 R) f.
+
+
+(*
+Lemma testing: 
+  forall a A B (P:a->A->Prop) (K:a->A->~~B->Prop) (f:val),
+  True ->
+  spec_1 (fun x R => forall X, P x X -> K x X R) f.
+Admitted.
+*)
+
 Lemma is_empty_spec : RepTotal is_empty (E;heap) >> 
   bool_of (E = \{}).
 Proof.
@@ -91,6 +130,7 @@ Fixpoint size h :=
   | Node a ho hs => (1 + size ho + size hs)%nat
   end.
 
+(*
 Lemma spec_induction_mut_2_2_2 : 
   forall A11 A12 B1 A21 A22 B2 (lt:binary(A11*A12+A21*A22)),
   forall (Wf: wf lt) f1 f2 (K1:A11->A12->~~B1->Prop) (K2:A21->A22->~~B2->Prop),
@@ -104,19 +144,50 @@ Lemma spec_induction_mut_2_2_2 :
     K2 x1 x2 R) f2 ->
   spec_2 K1 f1 /\ spec_2 K2 f2.
 Admitted.
+*)
 
+(*
 Definition link_spec := Spec link h1 h2 |R>>
-  forall x ho hs X Eo Es E2,
+  forall E1 E2,
+  inv h1 E1 ->
+  inv h2 E2 ->
+  forall x ho hs X Eo Es,
   h1 = Node x ho hs ->
   rep x X ->
   inv ho Eo ->
   inv hs Es ->
-  inv h2 E2 ->
   foreach (is_ge X) Eo ->
   foreach (is_ge X) Es ->
   foreach (is_ge X) E2 ->
   R (\{X} \u Eo \u Es \u E2 ; heap).
+*)
+(*
+Definition link_spec := RepSpec link (E1;heap) (E2;heap) |R>>
+  forall x h1 ho hs X Eo Es,
+  rep x X ->
+  inv ho Eo ->
+  inv hs Es ->
+  h1 = Node x ho hs ->
+  foreach (is_ge X) Eo ->
+  foreach (is_ge X) Es ->
+  foreach (is_ge X) E2 ->
+  R (\{X} \u Eo \u Es \u E2 ; heap).
+*)
 
+(*
+Definition is_rep_root X E :=
+  match E with
+  | Empty => False
+  | Node x ho hs => rep x X 
+  end.
+*)
+
+Definition link_spec := RepSpec link (E1;heap) (E2;heap) |R>>
+  forall X, min_of E1 X -> foreach (is_ge X) E2 ->
+  R (E1 \u E2 ; heap).
+
+
+(*
 Definition sum_measure A1 A2 (mu1:A1->nat) (mu2:A2->nat) (p:A1+A2) : nat :=
   match p with 
   | inl x => mu1 x 
@@ -126,82 +197,48 @@ Definition sum_measure A1 A2 (mu1:A1->nat) (mu2:A2->nat) (p:A1+A2) : nat :=
 
 Definition size_pair (p:heap*heap) :=
   let (h1,h2) := p in (size h1 + size h2)%nat.
-
-
-Lemma merge_spec : RepTotal merge (E1;heap) (E2;heap) >>
-  E1 \u E2 ; heap.
-Proof.
-  applys (>>> proj1 __ link_spec).
+*)
+(*
   sets lt: (fun p1 p2 => match p1,p2 with
     | inl x, inr y => size_pair x < size_pair y
     | inr x, inl y => size_pair x <= size_pair y
     | _,_ => False end).
-  eapply (spec_induction_mut_2_2_2 (lt:=lt)).
-   skip.
-  (* verif merge *)
-  xcf. introv _ IH R1 R2. subst lt. simpl in IH. xmatch; xcleanpat.
-  xgo. inverts R2. equates* 1.
-  xgo. inverts R1. equates* 1.
-  inverts R1. inverts R2. xapp~. xif.
-    xapp~. ximpl. equates* 1.
-    applys_to P_x0 nle_to_sle. xapp~. ximpl. equates* 1.
-  (* verif link *)
-  xcf. introv IH _ Sh1 Rx Ro Rs R2 Lo Ls L2. subst lt. simpl in IH.
-  xmatch; inverts H.
-  xgo. inverts Ro. constructors*. 
-  xgo~. skip. constructors*. (*todo: measure the models*)
-Qed.
-
-Hint Extern 1 (RegisterSpec merge) => Provide merge_spec.
-
-(* todo: simplify using rep_unique *)
-
-
-
-(*-- old
-
-Hint Extern 1 (RegisterSpec link) => Provide link_spec.
-
-Lemma merge_spec : RepTotal merge (E1;heap) (E2;heap) >>
-  E1 \u E2 ; heap.
-Proof.
-  xcf. introv R1 R2. xmatch; xcleanpat.
-  xgo. inverts R2. equates* 1.
-  xgo. inverts R1. equates* 1.
-  inverts R1. inverts R2. xapp~. xif.
-  xapp~. ximpl. equates* 1.
-  applys_to P_x0 nle_to_sle. xapp~. ximpl. equates* 1.
-Qed.
-
-Hint Extern 1 (RegisterSpec merge) => Provide merge_spec.
-
-Lemma link_spec : Spec link h1 h2 |R>>
-  forall x ho hs X Eo Es E2,
-  h1 = Node x ho hs ->
-  rep x X ->
-  inv ho Eo ->
-  inv hs Es ->
-  inv h2 E2 ->
-  foreach (is_ge X) Eo ->
-  foreach (is_ge X) Es ->
-  foreach (is_ge X) E2 ->
-  R (\{X} \u Eo \u Es \u E2 ; heap).
-Proof.
-  xcf. introv Sh1 Rx Ro Rs R2 Lo Ls L2.
-  xmatch; inverts H.
-  xgo. inverts Ro. constructors*.
-  xgo~. constructors*.
-Qed.
-
-Hint Extern 1 (RegisterSpec link) => Provide link_spec.
-
 *)
 
-Lemma insert_spec : RepTotal insert (X;O.t) (E;heap) >>
-  \{X} \u E ; heap.
-Proof. xgo~. ximpl. equates* 1. Qed.
 
-Hint Extern 1 (RegisterSpec insert) => Provide insert_spec.
+Axiom rep_induction_mut_2_2_2 : 
+  forall (a11 a12 A11 A12 B1 : Type)
+  (rep11:a11->A11->Prop) (rep12:a12->A12->Prop)
+  (mu1:A11->A12->nat) (RK1:a11->a12->A11->A12->~~B1->Prop) f1,
+  forall (a21 a22 A21 A22 B2 : Type)
+  (rep21:a21->A21->Prop) (rep22:a22->A22->Prop)
+  (mu2:A21->A22->nat) (RK2:a21->a22->A21->A22->~~B2->Prop) f2,
+  let IH := (fun n => 
+      rep_spec_2_hyp (B:=B1) rep11 rep12 (fun X11 X12 => (mu1 X11 X12 < n)%nat) RK1 f1
+   /\ rep_spec_2_hyp (B:=B2) rep21 rep22 (fun X21 X22 => (mu2 X21 X22 < n)%nat) RK2 f2) in
+  rep_spec_2_hyp (B:=B1) rep11 rep12 (fun X11 X12 => IH (mu1 X11 X12)) RK1 f1 -> 
+  rep_spec_2_hyp (B:=B2) rep21 rep22 (fun X21 X22 => IH (mu2 X21 X22)) RK2 f2 -> 
+     rep_spec_2 (B:=B1) rep11 rep12 RK1 f1 
+  /\ rep_spec_2 (B:=B2) rep21 rep22 RK2 f2.
+
+(*
+Lemma test : (BagEmpty (multiset T)).
+typeclass. Qed.
+Lemma test2 : (BagCard (multiset T)).
+typeclass. Qed.
+Lemma test23 : @card_empty (multiset T) _ _ _ = card_empty.
+typeclass. Qed.
+*)
+
+Hint Rewrite (card_empty (T:=multiset T)) (card_single (T:=multiset T))
+  (card_union (T:=multiset T)) : rew_card.
+Ltac rew_card := autorewrite with rew_card.
+
+Hint Extern 1 ((_ < _)%nat) => simpl; rew_card; math.
+
+Lemma is_ge_refl : forall x, is_ge x x.
+Proof. intros. apply le_refl. Qed.
+Hint Resolve is_ge_refl.
 
 Lemma min_of_prove : forall X Eo Es,
   foreach (is_ge X) Eo ->
@@ -213,6 +250,64 @@ Proof.
 Qed.
 
 Hint Resolve min_of_prove.
+
+
+Lemma min_of_eq : forall X Y E1 E2,
+  min_of (\{Y} \u E1 \u E2) X ->
+  foreach (is_ge Y) E1 ->
+  foreach (is_ge Y) E2 ->
+  Y <= X.
+Proof.
+  introv [M1 M2] G1 G2. multiset_in M1.
+  apply le_refl.
+  apply~ G1.
+  apply~ G2.
+Qed.
+
+(*
+Lemma min_of_eq : forall X Y E1 E2,
+  min_of (\{Y} \u E1 \u E2) X ->
+  foreach (is_ge X) E1 ->
+  foreach (is_ge X) E2 ->
+  X <= Y.
+Proof.
+  introv [M1 M2] G1 G2. multiset_in M1.
+  apply le_refl.
+  apply~ M2.
+  apply~ M2.
+Qed.
+*)
+
+Lemma merge_spec : RepTotal merge (E1;heap) (E2;heap) >>
+  E1 \u E2 ; heap.
+Proof.
+  applys (>>> proj1 __ link_spec).
+  eapply rep_induction_mut_2_2_2 with 
+   (mu1 := fun E1 E2 => (2 * (card E1 + card E2) + 1)%nat)
+   (mu2 := fun E1 E2 => (2 * (card E1 + card E2))%nat);
+   unfold rep_spec_2, rep_spec_2_hyp.
+  (* verif merge *)
+  xcf. introv R1 R2 [_ IH]. xmatch; xcleanpat.
+  xgo. inverts R2. equates* 1.
+  xgo. inverts R1. equates* 1.
+  inverts R1. inverts R2. xapp~. xif.
+    xapp~.
+    applys_to P_x0 nle_to_sle. xapp~. ximpl. equates* 1.
+  (* verif link *)
+  xcf. intros h1 h2 E1 E2 R1 R2 [IH _] X MX GX. inverts R1. 
+  xgo. applys_to MX proj1. eapply (in_empty X). eauto.
+  xmatch.
+  xgo. inverts H0. forwards~: (>>> min_of_eq MX). constructors*.
+  xgo~. forwards~: (>>> min_of_eq MX). constructors*.
+Qed.
+
+Hint Extern 1 (RegisterSpec merge) => Provide merge_spec.
+
+Lemma insert_spec : RepTotal insert (X;O.t) (E;heap) >>
+  \{X} \u E ; heap.
+Proof. xgo~. ximpl. equates* 1. Qed.
+
+Hint Extern 1 (RegisterSpec insert) => Provide insert_spec.
 
 Lemma find_min_spec : RepSpec find_min (E;heap) |R>>
   E <> \{} -> R (min_of E ;; O.t).
